correctness/RegexCorrectness/Backtracker/Basic.lean
@@ -13,7 +13,7 @@ namespace Regex.Backtracker
 namespace captureNextAux.pushNext
 
 variable {s : String} {σ : Strategy s} {nfa : NFA} {wf : nfa.WellFormed}
-  {startPos : Pos s} {stack : List (StackEntry σ nfa startPos)} {update : σ.Update} {state : Fin nfa.nodes.size} {pos : BVPos startPos}
+  {startPos : Pos s} {stack : List (StackEntry σ nfa startPos)} {update : σ.Update} {state : Fin nfa.size} {pos : BVPos startPos}
 
 theorem done (hn : nfa[state] = .done) : pushNext σ nfa wf startPos stack update state pos = stack := by
   rw! [pushNext, hn]
@@ -24,30 +24,30 @@ theorem fail (hn : nfa[state] = .fail) : pushNext σ nfa wf startPos stack updat
   rfl
 
 theorem epsilon {state' : Nat} (hn : nfa[state] = .epsilon state') :
-  haveI isLt : state' < nfa.nodes.size := wf.inBounds' state hn
+  haveI isLt : state' < nfa.size := wf.inBounds' state hn
   pushNext σ nfa wf startPos stack update state pos = ⟨update, ⟨state', isLt⟩, pos⟩ :: stack := by
   rw! [pushNext, hn]
   rfl
 
 theorem split {state₁ state₂ : Nat} (hn : nfa[state] = .split state₁ state₂) :
-  haveI isLt : state₁ < nfa.nodes.size ∧ state₂ < nfa.nodes.size := wf.inBounds' state hn
+  haveI isLt : state₁ < nfa.size ∧ state₂ < nfa.size := wf.inBounds' state hn
   pushNext σ nfa wf startPos stack update state pos = ⟨update, ⟨state₁, isLt.1⟩, pos⟩ :: ⟨update, ⟨state₂, isLt.2⟩, pos⟩ :: stack := by
   rw! [pushNext, hn]
   rfl
 
-theorem saveFin {offset : Nat} {state' : Fin nfa.nodes.size} (hn : nfa[state] = .save offset state') :
+theorem saveFin {offset : Nat} {state' : Fin nfa.size} (hn : nfa[state] = .save offset state') :
   pushNext σ nfa wf startPos stack update state pos = ⟨σ.write update offset pos.current, state', pos⟩ :: stack := by
   rw! [pushNext, hn]
   rfl
 
 theorem save {offset state' : Nat} (hn : nfa[state] = .save offset state') :
-  haveI isLt : state' < nfa.nodes.size := wf.inBounds' state hn
+  haveI isLt : state' < nfa.size := wf.inBounds' state hn
   pushNext σ nfa wf startPos stack update state pos = ⟨σ.write update offset pos.current, ⟨state', isLt⟩, pos⟩ :: stack := by
   rw! [pushNext, hn]
   rfl
 
 theorem anchor_pos {a : Data.Anchor} {state' : Nat} (hn : nfa[state] = .anchor a state') (h : Data.Anchor.test pos.current a) :
-  haveI isLt : state' < nfa.nodes.size := wf.inBounds' state hn
+  haveI isLt : state' < nfa.size := wf.inBounds' state hn
   pushNext σ nfa wf startPos stack update state pos = ⟨update, ⟨state', isLt⟩, pos⟩ :: stack := by
   rw! [pushNext, hn]
   simp [h]
@@ -58,7 +58,7 @@ theorem anchor_neg {a : Data.Anchor} {state' : Nat} (hn : nfa[state] = .anchor a
   simp [h]
 
 theorem char_pos {c : Char} {state' : Nat} (hn : nfa[state] = .char c state') (h : pos ≠ s.endBVPos startPos) (hc : pos.get h = c) :
-  haveI isLt : state' < nfa.nodes.size := wf.inBounds' state hn
+  haveI isLt : state' < nfa.size := wf.inBounds' state hn
   pushNext σ nfa wf startPos stack update state pos = ⟨update, ⟨state', isLt⟩, pos.next h⟩ :: stack := by
   rw! [pushNext, hn]
   simp [h, hc]
@@ -71,7 +71,7 @@ theorem char_neg {c : Char} {state' : Nat} (hn : nfa[state] = .char c state') (h
   | .inr ⟨ne, hc⟩ => simp [ne, hc]
 
 theorem sparse_pos {cs : Data.Classes} {state' : Nat} (hn : nfa[state] = .sparse cs state') (h : pos ≠ s.endBVPos startPos) (hc : pos.get h ∈ cs) :
-  haveI isLt : state' < nfa.nodes.size := wf.inBounds' state hn
+  haveI isLt : state' < nfa.size := wf.inBounds' state hn
   pushNext σ nfa wf startPos stack update state pos = ⟨update, ⟨state', isLt⟩, pos.next h⟩ :: stack := by
   rw! [pushNext, hn]
   simp [h, hc]
@@ -84,52 +84,52 @@ theorem sparse_neg {cs : Data.Classes} {state' : Nat} (hn : nfa[state] = .sparse
   | .inr ⟨ne, hc⟩ => simp [ne, hc]
 
 theorem fun_cases' (σ : Strategy s) (nfa : NFA) (wf : nfa.WellFormed) (startPos : Pos s)
-  {motive : List (StackEntry σ nfa startPos) → σ.Update → Fin nfa.nodes.size → BVPos startPos → Prop}
-  (done : ∀ (stack : List (StackEntry σ nfa startPos)) (update : σ.Update) (state : Fin nfa.nodes.size) (pos : BVPos startPos),
+  {motive : List (StackEntry σ nfa startPos) → σ.Update → Fin nfa.size → BVPos startPos → Prop}
+  (done : ∀ (stack : List (StackEntry σ nfa startPos)) (update : σ.Update) (state : Fin nfa.size) (pos : BVPos startPos),
     nfa[state] = .done → motive stack update state pos)
-  (fail : ∀ (stack : List (StackEntry σ nfa startPos)) (update : σ.Update) (state : Fin nfa.nodes.size) (pos : BVPos startPos),
+  (fail : ∀ (stack : List (StackEntry σ nfa startPos)) (update : σ.Update) (state : Fin nfa.size) (pos : BVPos startPos),
     nfa[state] = .fail → motive stack update state pos)
-  (epsilon : ∀ (stack : List (StackEntry σ nfa startPos)) (update : σ.Update) (state : Fin nfa.nodes.size) (pos : BVPos startPos) (state' : Fin nfa.nodes.size),
+  (epsilon : ∀ (stack : List (StackEntry σ nfa startPos)) (update : σ.Update) (state : Fin nfa.size) (pos : BVPos startPos) (state' : Fin nfa.size),
     nfa[state] = .epsilon state' → motive stack update state pos)
-  (split : ∀ (stack : List (StackEntry σ nfa startPos)) (update : σ.Update) (state : Fin nfa.nodes.size) (pos : BVPos startPos) (state₁ state₂ : Fin nfa.nodes.size),
+  (split : ∀ (stack : List (StackEntry σ nfa startPos)) (update : σ.Update) (state : Fin nfa.size) (pos : BVPos startPos) (state₁ state₂ : Fin nfa.size),
     nfa[state] = .split state₁ state₂ → motive stack update state pos)
-  (save : ∀ (stack : List (StackEntry σ nfa startPos)) (update : σ.Update) (state : Fin nfa.nodes.size) (pos : BVPos startPos) (offset : Nat) (state' : Fin nfa.nodes.size),
+  (save : ∀ (stack : List (StackEntry σ nfa startPos)) (update : σ.Update) (state : Fin nfa.size) (pos : BVPos startPos) (offset : Nat) (state' : Fin nfa.size),
     nfa[state] = .save offset state' → motive stack update state pos)
-  (anchor_pos : ∀ (stack : List (StackEntry σ nfa startPos)) (update : σ.Update) (state : Fin nfa.nodes.size) (pos : BVPos startPos) (a : Data.Anchor) (state' : Fin nfa.nodes.size),
+  (anchor_pos : ∀ (stack : List (StackEntry σ nfa startPos)) (update : σ.Update) (state : Fin nfa.size) (pos : BVPos startPos) (a : Data.Anchor) (state' : Fin nfa.size),
     nfa[state] = .anchor a state' → a.test pos.current → motive stack update state pos)
-  (anchor_neg : ∀ (stack : List (StackEntry σ nfa startPos)) (update : σ.Update) (state : Fin nfa.nodes.size) (pos : BVPos startPos) (a : Data.Anchor) (state' : Fin nfa.nodes.size),
+  (anchor_neg : ∀ (stack : List (StackEntry σ nfa startPos)) (update : σ.Update) (state : Fin nfa.size) (pos : BVPos startPos) (a : Data.Anchor) (state' : Fin nfa.size),
     nfa[state] = .anchor a state' → ¬a.test pos.current → motive stack update state pos)
-  (char_pos : ∀ (stack : List (StackEntry σ nfa startPos)) (update : σ.Update) (state : Fin nfa.nodes.size) (pos : BVPos startPos) (c : Char) (state' : Fin nfa.nodes.size),
+  (char_pos : ∀ (stack : List (StackEntry σ nfa startPos)) (update : σ.Update) (state : Fin nfa.size) (pos : BVPos startPos) (c : Char) (state' : Fin nfa.size),
     nfa[state] = .char c state' → (h : pos ≠ s.endBVPos startPos) → pos.get h = c → motive stack update state pos)
-  (char_neg : ∀ (stack : List (StackEntry σ nfa startPos)) (update : σ.Update) (state : Fin nfa.nodes.size) (pos : BVPos startPos) (c : Char) (state' : Fin nfa.nodes.size),
+  (char_neg : ∀ (stack : List (StackEntry σ nfa startPos)) (update : σ.Update) (state : Fin nfa.size) (pos : BVPos startPos) (c : Char) (state' : Fin nfa.size),
     nfa[state] = .char c state' → (pos = s.endBVPos startPos ∨ ∃ ne : pos ≠ s.endBVPos startPos, pos.get ne ≠ c) → motive stack update state pos)
-  (sparse_pos : ∀ (stack : List (StackEntry σ nfa startPos)) (update : σ.Update) (state : Fin nfa.nodes.size) (pos : BVPos startPos) (cs : Data.Classes) (state' : Fin nfa.nodes.size),
+  (sparse_pos : ∀ (stack : List (StackEntry σ nfa startPos)) (update : σ.Update) (state : Fin nfa.size) (pos : BVPos startPos) (cs : Data.Classes) (state' : Fin nfa.size),
     nfa[state] = .sparse cs state' → (h : pos ≠ s.endBVPos startPos) → pos.get h ∈ cs → motive stack update state pos)
-  (sparse_neg : ∀ (stack : List (StackEntry σ nfa startPos)) (update : σ.Update) (state : Fin nfa.nodes.size) (pos : BVPos startPos) (cs : Data.Classes) (state' : Fin nfa.nodes.size),
+  (sparse_neg : ∀ (stack : List (StackEntry σ nfa startPos)) (update : σ.Update) (state : Fin nfa.size) (pos : BVPos startPos) (cs : Data.Classes) (state' : Fin nfa.size),
     nfa[state] = .sparse cs state' → (pos = s.endBVPos startPos ∨ ∃ ne : pos ≠ s.endBVPos startPos, pos.get ne ∉ cs) → motive stack update state pos)
-  : ∀ (stack : List (StackEntry σ nfa startPos)) (update : σ.Update) (state : Fin nfa.nodes.size) (pos : BVPos startPos),
+  : ∀ (stack : List (StackEntry σ nfa startPos)) (update : σ.Update) (state : Fin nfa.size) (pos : BVPos startPos),
     motive stack update state pos :=
   fun stack update state pos =>
     match hn : nfa[state] with
     | .done => done stack update state pos hn
     | .fail => fail stack update state pos hn
     | .epsilon state' =>
-      have isLt : state' < nfa.nodes.size := wf.inBounds' state hn
+      have isLt : state' < nfa.size := wf.inBounds' state hn
       epsilon stack update state pos ⟨state', isLt⟩ hn
     | .split state₁ state₂ =>
-      have isLt : state₁ < nfa.nodes.size ∧ state₂ < nfa.nodes.size := wf.inBounds' state hn
+      have isLt : state₁ < nfa.size ∧ state₂ < nfa.size := wf.inBounds' state hn
       split stack update state pos ⟨state₁, isLt.1⟩ ⟨state₂, isLt.2⟩ hn
     | .save offset state' =>
-      have isLt : state' < nfa.nodes.size := wf.inBounds' state hn
+      have isLt : state' < nfa.size := wf.inBounds' state hn
       save stack update state pos offset ⟨state', isLt⟩ hn
     | .anchor a state' =>
-      have isLt : state' < nfa.nodes.size := wf.inBounds' state hn
+      have isLt : state' < nfa.size := wf.inBounds' state hn
       if ht : a.test pos.current then
         anchor_pos stack update state pos a ⟨state', isLt⟩ hn ht
       else
         anchor_neg stack update state pos a ⟨state', isLt⟩ hn ht
     | .char c state' =>
-      have isLt : state' < nfa.nodes.size := wf.inBounds' state hn
+      have isLt : state' < nfa.size := wf.inBounds' state hn
       if h : ∃ ne : pos ≠ s.endBVPos startPos, pos.get ne = c then
         char_pos stack update state pos c ⟨state', isLt⟩ hn h.1 h.2
       else
@@ -141,7 +141,7 @@ theorem fun_cases' (σ : Strategy s) (nfa : NFA) (wf : nfa.WellFormed) (startPos
             exact .inr ⟨ne, h⟩
         char_neg stack update state pos c ⟨state', isLt⟩ hn h'
     | .sparse cs state' =>
-      have isLt : state' < nfa.nodes.size := wf.inBounds' state hn
+      have isLt : state' < nfa.size := wf.inBounds' state hn
       if h : ∃ ne : pos ≠ s.endBVPos startPos, pos.get ne ∈ cs then
         sparse_pos stack update state pos cs ⟨state', isLt⟩ hn h.1 h.2
       else
@@ -156,22 +156,22 @@ theorem fun_cases' (σ : Strategy s) (nfa : NFA) (wf : nfa.WellFormed) (startPos
 end captureNextAux.pushNext
 
 theorem captureNextAux.induct' {s : String} (σ : Strategy s) (nfa : NFA) (wf : nfa.WellFormed) (startPos : Pos s)
-  (motive : BitMatrix nfa.nodes.size (startPos.remainingBytes + 1) → List (StackEntry σ nfa startPos) → Prop)
-  (base : ∀ (visited : BitMatrix nfa.nodes.size (startPos.remainingBytes + 1)), motive visited [])
-  (visited : ∀ (visited : BitMatrix nfa.nodes.size (startPos.remainingBytes + 1)) (update : σ.Update) (state : Fin nfa.nodes.size) (pos : BVPos startPos) (stack' : List (StackEntry σ nfa startPos)),
+  (motive : BitMatrix nfa.size (startPos.remainingBytes + 1) → List (StackEntry σ nfa startPos) → Prop)
+  (base : ∀ (visited : BitMatrix nfa.size (startPos.remainingBytes + 1)), motive visited [])
+  (visited : ∀ (visited : BitMatrix nfa.size (startPos.remainingBytes + 1)) (update : σ.Update) (state : Fin nfa.size) (pos : BVPos startPos) (stack' : List (StackEntry σ nfa startPos)),
     visited.get state pos.index →
     motive visited stack' →
     motive visited (⟨update, state, pos⟩ :: stack'))
-  (done : ∀ (visited : BitMatrix nfa.nodes.size (startPos.remainingBytes + 1)) (update : σ.Update) (state : Fin nfa.nodes.size) (pos : BVPos startPos) (stack' : List (StackEntry σ nfa startPos)),
+  (done : ∀ (visited : BitMatrix nfa.size (startPos.remainingBytes + 1)) (update : σ.Update) (state : Fin nfa.size) (pos : BVPos startPos) (stack' : List (StackEntry σ nfa startPos)),
     ¬visited.get state pos.index →
     nfa[state] = .done →
     motive visited (⟨update, state, pos⟩ :: stack'))
-  (next : ∀ (visited : BitMatrix nfa.nodes.size (startPos.remainingBytes + 1)) (update : σ.Update) (state : Fin nfa.nodes.size) (pos : BVPos startPos) (stack' : List (StackEntry σ nfa startPos)),
+  (next : ∀ (visited : BitMatrix nfa.size (startPos.remainingBytes + 1)) (update : σ.Update) (state : Fin nfa.size) (pos : BVPos startPos) (stack' : List (StackEntry σ nfa startPos)),
     ¬visited.get state pos.index →
     nfa[state] ≠ .done →
     motive (visited.set state pos.index) (pushNext σ nfa wf startPos stack' update state pos) →
     motive visited (⟨update, state, pos⟩ :: stack'))
-  : ∀ (visited : BitMatrix nfa.nodes.size (startPos.remainingBytes + 1)) (stack : List (StackEntry σ nfa startPos)), motive visited stack :=
+  : ∀ (visited : BitMatrix nfa.size (startPos.remainingBytes + 1)) (stack : List (StackEntry σ nfa startPos)), motive visited stack :=
   captureNextAux.induct σ nfa wf startPos motive
     base
     visited
@@ -183,7 +183,7 @@ Simplification lemmas for `captureNextAux`.
 -/
 section
 
-variable {s : String} {σ : Strategy s} {nfa : NFA} {wf : nfa.WellFormed} {startPos : Pos s} {visited : BitMatrix nfa.nodes.size (startPos.remainingBytes + 1)}
+variable {s : String} {σ : Strategy s} {nfa : NFA} {wf : nfa.WellFormed} {startPos : Pos s} {visited : BitMatrix nfa.size (startPos.remainingBytes + 1)}
 
 theorem captureNextAux_base :
   captureNextAux σ nfa wf startPos visited [] = (.none, visited) := by
@@ -215,20 +215,20 @@ theorem captureNextAux_next {update state pos stack'} (mem : ¬visited.get state
 end
 
 theorem captureNext.go.induct' {s : String} (σ : Strategy s) (nfa : NFA) (wf : nfa.WellFormed) (startPos : Pos s)
-  (motive : (pos : BVPos startPos) → BitMatrix nfa.nodes.size (startPos.remainingBytes + 1) → Prop)
-  (found : ∀ (pos : BVPos startPos) (visited : BitMatrix nfa.nodes.size (startPos.remainingBytes + 1)) (update : σ.Update) (visited' : BitMatrix nfa.nodes.size (startPos.remainingBytes + 1)),
+  (motive : (pos : BVPos startPos) → BitMatrix nfa.size (startPos.remainingBytes + 1) → Prop)
+  (found : ∀ (pos : BVPos startPos) (visited : BitMatrix nfa.size (startPos.remainingBytes + 1)) (update : σ.Update) (visited' : BitMatrix nfa.size (startPos.remainingBytes + 1)),
     captureNextAux σ nfa wf startPos visited [⟨σ.empty, ⟨nfa.start, wf.start_lt⟩, pos⟩] = (.some update, visited') →
     motive pos visited)
-  (not_found_next : ∀ (pos : BVPos startPos) (visited visited' : BitMatrix nfa.nodes.size (startPos.remainingBytes + 1)),
+  (not_found_next : ∀ (pos : BVPos startPos) (visited visited' : BitMatrix nfa.size (startPos.remainingBytes + 1)),
     captureNextAux σ nfa wf startPos visited [⟨σ.empty, ⟨nfa.start, wf.start_lt⟩, pos⟩] = (.none, visited') →
     (h : pos ≠ s.endBVPos startPos) →
     (ih : motive (pos.next h) visited') →
     motive pos visited)
-  (not_found_end : ∀ (pos : BVPos startPos) (visited visited' : BitMatrix nfa.nodes.size (startPos.remainingBytes + 1)),
+  (not_found_end : ∀ (pos : BVPos startPos) (visited visited' : BitMatrix nfa.size (startPos.remainingBytes + 1)),
     captureNextAux σ nfa wf startPos visited [⟨σ.empty, ⟨nfa.start, wf.start_lt⟩, pos⟩] = (.none, visited') →
     ¬pos ≠ s.endBVPos startPos →
     motive pos visited)
-  (pos : BVPos startPos) (visited : BitMatrix nfa.nodes.size (startPos.remainingBytes + 1)) :
+  (pos : BVPos startPos) (visited : BitMatrix nfa.size (startPos.remainingBytes + 1)) :
   motive pos visited :=
   captureNext.go.induct σ nfa wf startPos motive
     found not_found_next not_found_end pos visited
@@ -239,7 +239,7 @@ Simplification lemmas for `captureNext.go`.
 section
 
 variable {s : String} {σ : Strategy s} {nfa : NFA} {wf : nfa.WellFormed}
-  {startPos : Pos s} {visited : BitMatrix nfa.nodes.size (startPos.remainingBytes + 1)} {pos : BVPos startPos}
+  {startPos : Pos s} {visited : BitMatrix nfa.size (startPos.remainingBytes + 1)} {pos : BVPos startPos}
 
 theorem captureNext.go_found {update visited'} (h : captureNextAux σ nfa wf startPos visited [⟨σ.empty, ⟨nfa.start, wf.start_lt⟩, pos⟩] = (.some update, visited')) :
   captureNext.go σ nfa wf startPos pos visited = .some update := by
