correctness/RegexCorrectness/NFA/Semantics/ProofData/Cast.lean
@@ -14,13 +14,13 @@ namespace Group
 
 variable [Group] {s : String} {pos pos' : Pos s} {update}
 
-theorem castFromExpr (path : nfaExpr.Path nfaClose.nodes.size nfaExpr.start pos nfaClose.start pos' update) :
-  nfa'.Path nfaClose.nodes.size nfaExpr.start pos nfaClose.start pos' update := by
+theorem castFromExpr (path : nfaExpr.Path nfaClose.size nfaExpr.start pos nfaClose.start pos' update) :
+  nfa'.Path nfaClose.size nfaExpr.start pos nfaClose.start pos' update := by
   apply path.cast
   intro i _ lt
   exact ⟨Nat.lt_trans lt size_lt_expr', (get_lt_expr lt).symm⟩
 
-theorem castToExpr {lb j} (wf : nfa.WellFormed) (next_lt : next < nfa.nodes.size)
+theorem castToExpr {lb j} (wf : nfa.WellFormed) (next_lt : next < nfa.size)
   (path : nfa'.Path lb nfaExpr.start pos j pos' update) :
   nfaExpr.Path lb nfaExpr.start pos j pos' update := by
   have wf_expr := wf_expr wf next_lt
@@ -34,27 +34,27 @@ namespace Alternate
 
 variable [Alternate] {s : String} {pos pos' : Pos s} {update}
 
-theorem castFrom₁ (path : nfa₁.Path nfa.nodes.size nfa₁.start pos next pos' update) :
-  nfa'.Path nfa.nodes.size nfa₁.start pos next pos' update := by
+theorem castFrom₁ (path : nfa₁.Path nfa.size nfa₁.start pos next pos' update) :
+  nfa'.Path nfa.size nfa₁.start pos next pos' update := by
   apply path.cast
   intro i _ lt
   exact ⟨Nat.lt_trans lt size_lt₁, (get_lt₁ lt).symm⟩
 
-theorem castFrom₂ (path : nfa₂.Path nfa.nodes.size nfa₂.start pos next pos' update) :
-  nfa'.Path nfa.nodes.size nfa₂.start pos next pos' update := by
+theorem castFrom₂ (path : nfa₂.Path nfa.size nfa₂.start pos next pos' update) :
+  nfa'.Path nfa.size nfa₂.start pos next pos' update := by
   apply path.cast
   intro i _ lt
   exact ⟨Nat.lt_trans lt size_lt₂, (get_lt₂ lt).symm⟩
 
-theorem castTo₁ (wf : nfa.WellFormed) (next_lt : next < nfa.nodes.size)
-  (path : nfa'.Path nfa.nodes.size nfa₁.start pos next pos' update) :
-  nfa₁.Path nfa.nodes.size nfa₁.start pos next pos' update := by
+theorem castTo₁ (wf : nfa.WellFormed) (next_lt : next < nfa.size)
+  (path : nfa'.Path nfa.size nfa₁.start pos next pos' update) :
+  nfa₁.Path nfa.size nfa₁.start pos next pos' update := by
   have wf₁ := wf₁ wf next_lt
   apply path.cast' wf₁.start_lt (Nat.le_of_lt size_lt₁) wf₁
   intro i _ lt
   exact get_lt₁ lt
 
-theorem castTo₂ {lb} (wf : nfa.WellFormed) (next_lt : next < nfa.nodes.size)
+theorem castTo₂ {lb} (wf : nfa.WellFormed) (next_lt : next < nfa.size)
   (path : nfa'.Path lb nfa₂.start pos next pos' update) :
   nfa₂.Path lb nfa₂.start pos next pos' update := by
   have wf₂ := wf₂ wf next_lt
@@ -68,15 +68,15 @@ namespace Concat
 
 variable [Concat] {s : String} {pos pos' : Pos s} {update}
 
-theorem castFrom₂ (path : nfa₂.Path nfa.nodes.size nfa₂.start pos next pos' update) :
-  nfa'.Path nfa.nodes.size nfa₂.start pos next pos' update := by
+theorem castFrom₂ (path : nfa₂.Path nfa.size nfa₂.start pos next pos' update) :
+  nfa'.Path nfa.size nfa₂.start pos next pos' update := by
   apply path.cast
   intro i _ lt
   exact ⟨Nat.lt_trans lt size₂_lt, (get_lt₂ lt).symm⟩
 
-theorem castTo₂ (wf : nfa.WellFormed) (next_lt : next < nfa.nodes.size)
-  (path : nfa'.Path nfa.nodes.size nfa₂.start pos next pos' update) :
-  nfa₂.Path nfa.nodes.size nfa₂.start pos next pos' update := by
+theorem castTo₂ (wf : nfa.WellFormed) (next_lt : next < nfa.size)
+  (path : nfa'.Path nfa.size nfa₂.start pos next pos' update) :
+  nfa₂.Path nfa.size nfa₂.start pos next pos' update := by
   have wf₂ := wf₂ wf next_lt
   apply path.cast' wf₂.start_lt (Nat.le_of_lt size₂_lt) wf₂
   intro i _ lt
@@ -88,16 +88,16 @@ namespace Star
 
 variable [Star] {s : String} {pos pos' : Pos s} {update}
 
-theorem castFromExpr (path : nfaExpr.Path nfaPlaceholder.nodes.size nfaExpr.start pos nfaPlaceholder.start pos' update) :
-  nfa'.Path nfaPlaceholder.nodes.size nfaExpr.start pos nfaPlaceholder.start pos' update := by
+theorem castFromExpr (path : nfaExpr.Path nfaPlaceholder.size nfaExpr.start pos nfaPlaceholder.start pos' update) :
+  nfa'.Path nfaPlaceholder.size nfaExpr.start pos nfaPlaceholder.start pos' update := by
   apply path.cast
   intro i ge lt
   simp [nfaPlaceholder] at ge
   exact ⟨size_eq_expr' ▸ lt, (get_ne_start i (size_eq_expr' ▸ lt) (Nat.ne_of_gt ge)).symm⟩
 
 theorem castToExpr (wf : nfa.WellFormed)
-  (path : nfa'.Path nfaPlaceholder.nodes.size nfaExpr.start pos nfaPlaceholder.start pos' update) :
-  nfaExpr.Path nfaPlaceholder.nodes.size nfaExpr.start pos nfaPlaceholder.start pos' update := by
+  (path : nfa'.Path nfaPlaceholder.size nfaExpr.start pos nfaPlaceholder.start pos' update) :
+  nfaExpr.Path nfaPlaceholder.size nfaExpr.start pos nfaPlaceholder.start pos' update := by
   have wf_expr := wf_expr wf
   apply path.cast' wf_expr.start_lt (Nat.le_of_eq size_eq_expr'.symm) wf_expr
   intro i ge lt
