correctness/RegexCorrectness/NFA/Semantics/ProofData/Compile.lean
@@ -14,33 +14,33 @@ variable {s : String} {nfa : NFA} {next e result lb} {pos pos' : Pos s} {i j upd
 
 @[grind →]
 theorem Step.eq_or_lt_of_pushNode {node} (step : (nfa.pushNode node).Step lb i pos j pos' update) :
-  i = nfa.nodes.size ∨ i < nfa.nodes.size ∧ nfa.Step lb i pos j pos' update := by
+  i = nfa.size ∨ i < nfa.size ∧ nfa.Step lb i pos j pos' update := by
   grind
 
 @[grind →]
 theorem Step.eq_or_lt_of_pushRegex (step : (nfa.pushRegex next e).Step lb i pos j pos' update) :
-  nfa.nodes.size ≤ i ∨ i < nfa.nodes.size ∧ nfa.Step lb i pos j pos' update := by
+  nfa.size ≤ i ∨ i < nfa.size ∧ nfa.Step lb i pos j pos' update := by
   fun_induction pushRegex <;> grind [pushRegex_size_lt]
 
 @[grind →]
 theorem Step.eq_or_ge_of_pushRegex
-  (step : (nfa.pushRegex next e).Step nfa.nodes.size i pos j pos' update) :
-  j = next ∨ nfa.nodes.size ≤ j := by
-  fun_induction pushRegex <;> grind [pushRegex_size_lt]
+  (step : (nfa.pushRegex next e).Step nfa.size i pos j pos' update) :
+  j = next ∨ nfa.size ≤ j := by
+  fun_induction pushRegex <;> grind [pushRegex_size_lt, NFA.size]
 
 theorem Path.eq_or_path_next (eq : nfa.pushRegex next e = result)
-  (jlt : j < nfa.nodes.size) (ige : i ≥ nfa.nodes.size)
+  (jlt : j < nfa.size) (ige : i ≥ nfa.size)
   (path : result.Path lb i pos j pos' update) :
   j = next ∨
   ∃ posm update₁ update₂,
     update = update₁ ++ update₂ ∧
-    result.Path nfa.nodes.size i pos next posm update₁ ∧
+    result.Path nfa.size i pos next posm update₁ ∧
     result.Path lb next posm j pos' update₂ := by
   induction path with
   | @last i pos j pos' update step =>
     have step := eq ▸ step.liftBound' ige
     have := step.eq_or_ge_of_pushRegex
-    omega
+    grind [NFA.size]
   | @more i pos j pos' k pos'' update updates step rest ih =>
     have step := step.liftBound' ige
     cases (eq ▸ step).eq_or_ge_of_pushRegex with
@@ -54,11 +54,11 @@ theorem Path.eq_or_path_next (eq : nfa.pushRegex next e = result)
         exact .inr ⟨itm, update ::ₒ update₁, update₂, by simp [equ], .more step path₁, path₂⟩
 
 theorem Path.path_next_of_ne (eq : nfa.pushRegex next e = result)
-  (jlt : j < nfa.nodes.size) (ige : i ≥ nfa.nodes.size) (ne : j ≠ next)
+  (jlt : j < nfa.size) (ige : i ≥ nfa.size) (ne : j ≠ next)
   (path : result.Path lb i pos j pos' update) :
   ∃ posm update₁ update₂,
     update = update₁ ++ update₂ ∧
-    result.Path nfa.nodes.size i pos next posm update₁ ∧
+    result.Path nfa.size i pos next posm update₁ ∧
     result.Path lb next posm j pos' update₂ := by
   have := path.eq_or_path_next eq jlt ige
   cases this with
