regex/Regex/NFA/Compile/Lemmas.lean
@@ -6,7 +6,7 @@ import all Regex.NFA.Compile.Basic
 namespace Regex.NFA
 
 public theorem pushRegex_size_lt {nfa : NFA} {next e} :
-  nfa.nodes.size < (nfa.pushRegex next e).nodes.size := by
+  nfa.size < (nfa.pushRegex next e).size := by
   induction e generalizing nfa next with
   | empty => simp [pushRegex]
   | epsilon => simp [pushRegex]
@@ -15,25 +15,25 @@ public theorem pushRegex_size_lt {nfa : NFA} {next e} :
   | classes => simp [pushRegex]
   | group tag e ih =>
     simp [pushRegex]
-    calc nfa.nodes.size
-      _ < (nfa.pushNode (.save (2 * tag + 1) next)).nodes.size := by simp
-      _ < ((nfa.pushNode (.save (2 * tag + 1) next)).pushRegex nfa.nodes.size e).nodes.size := ih
+    calc nfa.size
+      _ < (nfa.pushNode (.save (2 * tag + 1) next)).size := by simp
+      _ < ((nfa.pushNode (.save (2 * tag + 1) next)).pushRegex nfa.size e).size := ih
       _ < _ := by omega
   | alternate e₁ e₂ ih₁ ih₂ =>
     simp [pushRegex]
-    calc nfa.nodes.size
-      _ < (nfa.pushRegex next e₁).nodes.size := ih₁
-      _ < ((nfa.pushRegex next e₁).pushRegex next e₂).nodes.size := ih₂
+    calc nfa.size
+      _ < (nfa.pushRegex next e₁).size := ih₁
+      _ < ((nfa.pushRegex next e₁).pushRegex next e₂).size := ih₂
       _ < _ := by omega
   | concat e₁ e₂ ih₁ ih₂ =>
     simp [pushRegex]
-    calc nfa.nodes.size
-      _ < (nfa.pushRegex next e₂).nodes.size := ih₂
+    calc nfa.size
+      _ < (nfa.pushRegex next e₂).size := ih₂
       _ < _ := ih₁
   | star greedy e ih =>
-    simp [pushRegex]
-    calc nfa.nodes.size
-      _ < (nfa.pushNode .fail).nodes.size := by simp
-      _ < ((nfa.pushNode .fail).pushRegex nfa.nodes.size e).nodes.size := ih
+    simp [pushRegex, size]
+    calc nfa.size
+      _ < (nfa.pushNode .fail).size := by simp
+      _ < ((nfa.pushNode .fail).pushRegex nfa.size e).size := ih
 
 end Regex.NFA
